fix: also generate document when text is empty (#402)

examples/website-examples/AnchorExamples.lean
@@ -7,29 +7,32 @@ import Examples.Basic
 
 
 -- ANCHOR: t
-def t : Tree Nat :=
+def someTree : Tree Nat :=
 -- ANCHOR: tDef
   .branch (.branch .leaf 1 .leaf) 2 (.branch (.branch .leaf 3 .leaf) 4 .leaf)
 -- ANCHOR_END: tDef
 -- ANCHOR_END: t
 
-example := t.flip
+example := someTree.flip
 
+deriving instance Repr for Tree
 
 -- ANCHOR: tflip
-#check Tree.flip
+#eval someTree.flip
 -- ANCHOR_END: tflip
 
 
 
 
 -- ANCHOR: proof1
-theorem Tree.flip_flip_id (t : Tree α) : t.flip.flip = t := by
+theorem Tree.flip_flip_eq_id : flip ∘ flip = (id : Tree α → Tree α) := by
+  funext t
   induction t with
   | leaf => rfl
+-- ANCHOR: proof1a
   | branch l v r ih1 ih2 =>
-    simp only [flip]
-    rw [ih1]; rw [ih2]
+    simp_all [flip]
+-- ANCHOR_END: proof1a
 -- ANCHOR_END: proof1
 
 -- ANCHOR: proof2
